erasure/theories/EOptimizePropDiscr.v
@@ -31,6 +31,27 @@ Set Warnings "-notation-overridden".
 Import E.
 Set Warnings "+notation-overridden".
 
+
+Lemma closedn_subst s k t : 
+  forallb (closedn k) s -> closedn (#|s| + k) t -> 
+  closedn k (subst0 s t).
+Proof. Admitted.
+
+Lemma closed_csubst t k u : 
+  closedn k t -> 
+  closedn (S k) u -> 
+  closedn k (ECSubst.csubst t 0 u).
+Proof.
+  intros.
+Admitted.
+
+Lemma closed_substl ts k u : 
+  forallb (closedn k) ts -> 
+  closedn (#|ts| + k) u -> 
+  closedn k (ECSubst.substl ts u).
+Proof.
+  intros.
+Admitted.
 Section optimize.
   Context (Σ : global_context).
 
@@ -46,7 +67,7 @@ Section optimize.
       match ETyping.is_propositional_ind Σ (fst ind) with
       | Some true =>
         match brs' with
-        | [(a, b)] => E.mkApps b (repeat E.tBox a)
+        | [(a, b)] => ECSubst.substl (repeat E.tBox a) b
         | _ => E.tCase ind (optimize c) brs'
         end
       | _ => E.tCase ind (optimize c) brs'
@@ -74,16 +95,7 @@ Section optimize.
     induction l using rev_ind; simpl; auto.
     now rewrite -mkApps_nested /= IHl map_app /= -mkApps_nested /=.
   Qed.
-  
-  Lemma optimize_iota_red pars n args brs :
-    optimize (ETyping.iota_red pars n args brs) = ETyping.iota_red pars n (map optimize args) (map (on_snd optimize) brs).
-  Proof.
-    unfold ETyping.iota_red.
-    rewrite !nth_nth_error nth_error_map.
-    destruct nth_error eqn:hnth => /=;
-    now rewrite optimize_mkApps map_skipn.
-  Qed.
-  
+
   Lemma map_repeat {A B} (f : A -> B) x n : map f (repeat x n) = repeat (f x) n.
   Proof.
     now induction n; simpl; auto; rewrite IHn.
@@ -101,49 +113,137 @@ Section optimize.
     now rewrite [EAst.tApp _ _](mkApps_nested _ _ [_]) map_app.
   Qed.
 
+  Lemma csubst_closed t k x : closedn k x -> csubst t k x = x.
+  Proof.
+    induction x in k |- * using EInduction.term_forall_list_ind; simpl; auto.
+    all:try solve [intros; f_equal; solve_all; eauto].
+    intros Hn. eapply Nat.ltb_lt in Hn.
+    - destruct (Nat.compare_spec k n); try lia. reflexivity.
+    - move/andP => []. intros. f_equal; solve_all; eauto.
+    - move/andP => []. intros. f_equal; solve_all; eauto.
+    - move/andP => []. intros. f_equal; solve_all; eauto.
+      destruct x0; cbn in *. f_equal; auto.
+  Qed.
+
+
+  Lemma closed_optimize t k : closedn k t -> closedn k (optimize t).
+  Proof.
+    induction t in k |- * using EInduction.term_forall_list_ind; simpl; auto;
+    intros; try easy;
+    rewrite -> ?map_map_compose, ?compose_on_snd, ?compose_map_def, ?map_length;
+    unfold test_def in *;
+    simpl closed in *; try solve [simpl subst; simpl closed; f_equal; auto; rtoProp; solve_all]; try easy.
+    - move/andP: H => [] clt cll. destruct ETyping.is_propositional_ind as [[|]|] => /= //.
+      destruct l as [|[br n] [|l']] eqn:eql; simpl.
+      rewrite IHt //.
+      depelim X. cbn in *.
+      rewrite andb_true_r in cll.
+      specialize (i _ cll).
+      eapply closed_substl. solve_all. eapply All_repeat => //.
+      now rewrite repeat_length.
+      rtoProp; solve_all. depelim cll. solve_all.
+      depelim cll. depelim cll. solve_all.
+      depelim cll. depelim cll. solve_all.
+      rtoProp; solve_all. solve_all.
+      rtoProp; solve_all. solve_all.
+    - destruct ETyping.is_propositional_ind.
+      destruct b => //. cbn; auto.
+      cbn; auto.
+  Qed.
+ 
+  Lemma subst_csubst_comm l t k b : 
+    forallb (closedn 0) l -> closed t ->
+    subst l 0 (csubst t (#|l| + k) b) = 
+    csubst t k (subst l 0 b).
+  Proof.
+    intros hl cl.
+    rewrite !closed_subst //.
+    rewrite distr_subst. f_equal.
+    symmetry. solve_all.
+    rewrite subst_closed //.
+    eapply closed_upwards; tea. lia. 
+  Qed.
+
+  Lemma substl_subst s t : 
+    forallb (closedn 0) s ->
+    substl s t = subst s 0 t.
+  Proof.
+    induction s in t |- *; cbn; auto.
+    intros _. now rewrite subst_empty.
+    move/andP=> []cla cls.
+    rewrite (subst_app_decomp [_]).
+    cbn. rewrite lift_closed //.
+    rewrite closed_subst //. now eapply IHs.
+  Qed.
+
+  Lemma substl_csubst_comm l t k b : 
+    forallb (closedn 0) l -> closed t ->
+    substl l (csubst t (#|l| + k) b) = 
+    csubst t k (substl l b).
+  Proof.
+    intros hl cl.
+    rewrite substl_subst //.
+    rewrite substl_subst //.
+    apply subst_csubst_comm => //.
+  Qed.
+
   Lemma optimize_csubst a k b : 
+    closed a ->
     optimize (ECSubst.csubst a k b) = ECSubst.csubst (optimize a) k (optimize b).
   Proof.
-    induction b in k |- * using EInduction.term_forall_list_ind; simpl; auto; 
-      try solve [f_equal; eauto; ELiftSubst.solve_all].
-    
+    induction b in k |- * using EInduction.term_forall_list_ind; simpl; auto;
+    intros; try easy;
+    rewrite -> ?map_map_compose, ?compose_on_snd, ?compose_map_def, ?map_length;
+    unfold test_def in *;
+    simpl closed in *; try solve [simpl subst; simpl closed; f_equal; auto; rtoProp; solve_all]; try easy.
     - destruct (k ?= n); auto.
-    - f_equal; eauto. rewrite !map_map_compose; eauto.
-      solve_all.
     - destruct ETyping.is_propositional_ind as [[|]|] => /= //.
       destruct l as [|[br n] [|l']] eqn:eql; simpl.
       * f_equal; auto.
       * depelim X. simpl in *.
-        rewrite e. rewrite csubst_mkApps.
-        now rewrite map_repeat /=.
-      * depelim X.
-        f_equal; eauto.
-        f_equal; eauto. now rewrite e.
-        f_equal; eauto.
-        f_equal. depelim X.
-        now rewrite e0. depelim X. rewrite !map_map_compose.
-        solve_all.
-      * f_equal; eauto.
-        rewrite !map_map_compose; solve_all.
-      * f_equal; eauto.
-        rewrite !map_map_compose; solve_all.
+        rewrite e //.
+        assert (br = #|repeat tBox br|). now rewrite repeat_length.
+        rewrite {2}H0.
+        rewrite substl_csubst_comm //.
+        solve_all. eapply All_repeat => //.
+        now eapply closed_optimize.
+      * depelim X. depelim X.
+        f_equal; eauto. f_equal; eauto. f_equal; eauto.
+        f_equal; eauto. f_equal; eauto.
+        rewrite map_map_compose; solve_all.
+      * rewrite ?map_map_compose; f_equal; eauto; solve_all.
+      * rewrite ?map_map_compose; f_equal; eauto; solve_all.
     - destruct ETyping.is_propositional_ind as [[|]|]=> //;
       now rewrite IHb.
-    - rewrite !map_map_compose; f_equal; solve_all.
+    - f_equal; solve_all.
       destruct x; unfold EAst.map_def; simpl in *. 
       autorewrite with len. f_equal; eauto.
-    - rewrite !map_map_compose; f_equal; solve_all.
+    - f_equal; solve_all.
       destruct x; unfold EAst.map_def; simpl in *. 
       autorewrite with len. f_equal; eauto.
   Qed.
 
-  Lemma optimize_substl s t : optimize (Ee.substl s t) = Ee.substl (map optimize s) (optimize t).
+  Lemma optimize_substl s t : 
+    forallb (closedn 0) s ->
+    optimize (substl s t) = substl (map optimize s) (optimize t).
   Proof.
     induction s in t |- *; simpl; auto.
-    rewrite IHs. f_equal.
+    move/andP => [] cla cls.
+    rewrite IHs //. f_equal.
     now rewrite optimize_csubst.
   Qed.
 
+  Lemma optimize_iota_red pars args br :
+    forallb (closedn 0) args ->
+    optimize (ETyping.iota_red pars args br) = ETyping.iota_red pars (map optimize args) (on_snd optimize br).
+  Proof.
+    intros cl.
+    unfold ETyping.iota_red.
+    rewrite optimize_substl //.
+    rewrite forallb_skipn //.
+    now rewrite map_skipn.
+  Qed.
+  
   Lemma optimize_fix_subst mfix : ETyping.fix_subst (map (map_def optimize) mfix) = map optimize (ETyping.fix_subst mfix).
   Proof.
     unfold ETyping.fix_subst.
@@ -163,26 +263,30 @@ Section optimize.
   Qed.
 
   Lemma optimize_cunfold_fix mfix idx n f : 
+    forallb (closedn 0) (ETyping.fix_subst mfix) ->
     Ee.cunfold_fix mfix idx = Some (n, f) ->
     Ee.cunfold_fix (map (map_def optimize) mfix) idx = Some (n, optimize f).
   Proof.
+    intros hfix.
     unfold Ee.cunfold_fix.
     rewrite nth_error_map.
     destruct nth_error.
     intros [= <- <-] => /=. f_equal.
-    now rewrite optimize_substl optimize_fix_subst.
+    now rewrite optimize_substl // optimize_fix_subst.
     discriminate.
   Qed.
 
   Lemma optimize_cunfold_cofix mfix idx n f : 
+    forallb (closedn 0) (ETyping.cofix_subst mfix) ->
     Ee.cunfold_cofix mfix idx = Some (n, f) ->
     Ee.cunfold_cofix (map (map_def optimize) mfix) idx = Some (n, optimize f).
   Proof.
+    intros hcofix.
     unfold Ee.cunfold_cofix.
     rewrite nth_error_map.
     destruct nth_error.
     intros [= <- <-] => /=. f_equal.
-    now rewrite optimize_substl optimize_cofix_subst.
+    now rewrite optimize_substl // optimize_cofix_subst.
     discriminate.
   Qed.
 
@@ -372,73 +476,227 @@ Proof.
   red in isdecl |- *. eauto using extends_lookup.
 Qed.
 
+Lemma closedn_mkApps k f args : closedn k (mkApps f args) = closedn k f && forallb (closedn k) args.
+Proof.
+  induction args in f |- *; simpl; auto.
+  ring. rewrite IHargs /=. ring. 
+Qed.
+
+(** Evaluation preserves closedness: *)
+Lemma eval_closed {wfl : Ee.WcbvFlags} Σ : forall t u, closed t -> Ee.eval Σ t u -> closed u.
+Proof.
+  move=> t u Hc ev. move: Hc.
+  induction ev; simpl in *; auto;
+    (move/andP=> [/andP[Hc Hc'] Hc''] || move/andP=> [Hc Hc'] || move=>Hc); auto.
+  - eapply IHev3. rewrite ECSubst.closed_subst //. auto.
+    eapply closedn_subst; tea. cbn. rewrite andb_true_r. auto. cbn. auto.
+  - eapply IHev2.
+    rewrite ECSubst.closed_subst; auto.
+    eapply closedn_subst; tea. cbn. rewrite andb_true_r. auto.
+  - apply IHev2. todo "case".
+  - eapply IHev2. solve_all.
+    todo "case".
+  - eapply IHev3.
+    apply/andP.
+    split; [|easy].
+    specialize (IHev1 Hc).
+    rewrite closedn_mkApps in IHev1.
+    move/andP: IHev1 => [clfix clargs].
+    rewrite closedn_mkApps clargs andb_true_r.
+    todo "case".
+    (* eapply closed_unfold_fix; [easy|]. *)
+    (* now rewrite closed_unfold_fix_cunfold_eq. *)
+  - apply andb_true_iff.
+    split; [|easy].
+    solve_all.
+  - eapply IHev. rewrite closedn_mkApps.
+    rewrite closedn_mkApps in Hc. move/andP: Hc => [Hfix Hargs].
+    repeat (apply/andP; split; auto). 
+    todo "case".
+     (* rewrite -closed_unfold_cofix_cunfold_eq in e => //. *)
+    (* eapply closed_unfold_cofix in e; eauto. *)
+  - eapply IHev. rewrite closedn_mkApps in Hc *.
+    move/andP: Hc => [Hfix Hargs].
+    rewrite closedn_mkApps Hargs.
+    todo "casE".
+    (* rewrite -closed_unfold_cofix_cunfold_eq in e => //.
+    eapply closed_unfold_cofix in e; eauto.
+    now rewrite e. *)
+  - apply IHev. todo "case".
+  - todo "case".
+  - rtoProp; intuition auto.
+Qed.
+
+Lemma closed_iota_red pars c args brs br :
+  forallb (closedn 0) args ->
+  nth_error brs c = Some br ->
+  #|skipn pars args| = br.1 ->
+  closedn br.1 br.2 ->
+  closed (iota_red pars args br).
+Proof.
+  intros clargs hnth hskip clbr.
+  rewrite /iota_red.
+  eapply closed_substl => //.
+  now rewrite forallb_skipn.
+  now rewrite hskip Nat.add_0_r.
+Qed.
+
+Lemma closed_fix_subst mfix idx : 
+  closed (EAst.tFix mfix idx) ->
+  forallb (closedn 0) (fix_subst mfix).
+Proof. Admitted.
+
+Lemma closed_cofix_subst mfix idx : 
+  closed (EAst.tCoFix mfix idx) ->
+  forallb (closedn 0) (cofix_subst mfix).
+Proof. Admitted.
+
+Lemma closed_cunfold_fix mfix idx n f : 
+  closed (EAst.tFix mfix idx) ->
+  Ee.cunfold_fix mfix idx = Some (n, f) ->
+  closed f.
+Proof.
+  move=> cl.
+  rewrite /Ee.cunfold_fix.
+  destruct nth_error eqn:heq => //.
+  cbn in cl.
+  have := (nth_error_forallb heq cl) => cld. 
+  move=> [=] _ <-.
+  eapply closed_substl. now eapply (closed_fix_subst _ idx).
+  rewrite fix_subst_length.
+  apply cld.
+Qed.
+
+Lemma closed_cunfold_cofix mfix idx n f : 
+  closed (EAst.tCoFix mfix idx) ->
+  Ee.cunfold_cofix mfix idx = Some (n, f) ->
+  closed f.
+Proof.
+  move=> cl.
+  rewrite /Ee.cunfold_cofix.
+  destruct nth_error eqn:heq => //.
+  cbn in cl.
+  have := (nth_error_forallb heq cl) => cld. 
+  move=> [=] _ <-.
+  eapply closed_substl. now eapply (closed_cofix_subst _ idx).
+  rewrite cofix_subst_length.
+  apply cld.
+Qed.
+
 Lemma optimize_correct Σ t v :
   @Ee.eval Ee.default_wcbv_flags Σ t v ->
+  closed t ->
   @Ee.eval Ee.opt_wcbv_flags (optimize_env Σ) (optimize Σ t) (optimize Σ v).
 Proof.
   intros ev.
   induction ev; simpl in *; try solve [econstructor; eauto].
 
-  - econstructor; eauto.
-    now rewrite optimize_csubst in IHev3.
+  - move/andP => [] cla clt. econstructor; eauto.
+  - move/andP => [] clf cla. econstructor; eauto.
+    rewrite optimize_csubst in IHev3.
+    now eapply eval_closed in ev2.
+    apply IHev3. todo "casE".
 
-  - rewrite optimize_csubst in IHev2.
-    econstructor; eauto.
+  - move/andP => [] clb0 clb1. rewrite optimize_csubst in IHev2.
+    now eapply eval_closed in ev1.
+    econstructor; eauto. eapply IHev2, closed_csubst => //.
+    now eapply eval_closed in ev1.
 
-  - rewrite optimize_mkApps in IHev1.
+  - move/andP => [] cld clbrs. rewrite optimize_mkApps in IHev1.
+    have := (eval_closed _ _ _ cld ev1); rewrite closedn_mkApps => /andP[] _ clargs.
     rewrite optimize_iota_red in IHev2.
+    eapply eval_closed in ev1 => //.
     destruct ETyping.is_propositional_ind as [[]|]eqn:isp => //.
     eapply Ee.eval_iota; eauto.
     now rewrite -is_propositional_optimize.
+    rewrite nth_error_map e0 //. now len.
+    eapply IHev2.
+    eapply closed_iota_red => //; tea.
+    eapply nth_error_forallb in clbrs; tea. cbn in clbrs.
+    now rewrite Nat.add_0_r in clbrs.
   
-  - rewrite e e0 /=.
-    now rewrite optimize_mkApps map_optimize_repeat_box in IHev2.
+  - move/andP => [] cld clbrs. rewrite e e0 /=.
+    subst brs. cbn in clbrs. rewrite Nat.add_0_r andb_true_r in clbrs.
+    rewrite optimize_substl in IHev2. 
+    eapply All_forallb, All_repeat => //.
+    rewrite map_optimize_repeat_box in IHev2.
+    apply IHev2.
+    eapply closed_substl.
+    eapply All_forallb, All_repeat => //.
+    now rewrite repeat_length Nat.add_0_r.
 
-  - rewrite optimize_mkApps in IHev1.
-    simpl in *. eapply Ee.eval_fix; eauto.
-    rewrite map_length. now eapply optimize_cunfold_fix. 
-    now rewrite optimize_mkApps in IHev3.
+  - move/andP => [] clf cla. rewrite optimize_mkApps in IHev1.
+    simpl in *.
+    eapply eval_closed in ev1 => //.
+    rewrite closedn_mkApps in ev1.
+    move: ev1 => /andP [] clfix clargs.
+    eapply Ee.eval_fix; eauto.
+    rewrite map_length.
+    eapply optimize_cunfold_fix; tea.
+    now eapply closed_fix_subst.
+    rewrite optimize_mkApps in IHev3. apply IHev3.
+    rewrite closedn_mkApps clargs.
+    eapply eval_closed in ev2; tas. rewrite ev2 /= !andb_true_r.
+    eapply closed_cunfold_fix; tea.
 
-  - rewrite optimize_mkApps in IHev1 |- *.
+  - move/andP => [] clf cla.
+    eapply eval_closed in ev1 => //.
+    rewrite closedn_mkApps in ev1.
+    move: ev1 => /andP [] clfix clargs.
+    eapply eval_closed in ev2; tas.
+    rewrite optimize_mkApps in IHev1 |- *.
     simpl in *. eapply Ee.eval_fix_value. auto. auto.
-    eapply optimize_cunfold_fix; eauto. now rewrite map_length. 
+    eapply optimize_cunfold_fix; eauto.
+    eapply closed_fix_subst => //.
+    now rewrite map_length. 
 
-  - destruct ETyping.is_propositional_ind as [[]|] eqn:isp => //.
+  - move/andP => []. rewrite closedn_mkApps. move/andP => [] clfix clargs clbrs.
+    forward IHev.
+    { rewrite closedn_mkApps clargs clbrs !andb_true_r.
+      eapply closed_cunfold_cofix; tea. }
+    destruct ETyping.is_propositional_ind as [[]|] eqn:isp => //.
     destruct brs as [|[a b] []]; simpl in *; auto.
     rewrite -> optimize_mkApps in IHev |- *. simpl.
     econstructor; eauto.
-    now apply optimize_cunfold_cofix.
+    apply optimize_cunfold_cofix; tea. eapply closed_cofix_subst; tea.
+    
     rewrite -> optimize_mkApps in IHev |- *. simpl.
     econstructor; eauto.
-    now apply optimize_cunfold_cofix.
+    apply optimize_cunfold_cofix; tea. eapply closed_cofix_subst; tea.
     rewrite -> optimize_mkApps in IHev |- *. simpl.
     econstructor; eauto.
-    now apply optimize_cunfold_cofix.
+    apply optimize_cunfold_cofix; tea. eapply closed_cofix_subst; tea.
     rewrite -> optimize_mkApps in IHev |- *. simpl.
     econstructor; eauto.
-    now apply optimize_cunfold_cofix.
+    apply optimize_cunfold_cofix; tea. eapply closed_cofix_subst; tea.
 
-  - destruct ETyping.is_propositional_ind as [[]|] eqn:isp; auto.
+  - rewrite closedn_mkApps; move/andP => [] clfix clargs. forward IHev.
+    { rewrite closedn_mkApps clargs andb_true_r. eapply closed_cunfold_cofix; tea. }
+    destruct ETyping.is_propositional_ind as [[]|] eqn:isp; auto.
     rewrite -> optimize_mkApps in IHev |- *. simpl.
     econstructor; eauto.
-    now apply optimize_cunfold_cofix.
+    apply optimize_cunfold_cofix; tea. eapply closed_cofix_subst; tea.
     rewrite -> optimize_mkApps in IHev |- *. simpl.
     econstructor; eauto.
-    now apply optimize_cunfold_cofix.
+    apply optimize_cunfold_cofix; tea. eapply closed_cofix_subst; tea.
   
   - econstructor. red in isdecl |- *.
     rewrite lookup_env_optimize isdecl //.
     now rewrite /optimize_constant_decl e.
     apply IHev.
+    admit.
   
   - destruct ETyping.is_propositional_ind as [[]|] eqn:isp => //.
     rewrite optimize_mkApps in IHev1.
     rewrite optimize_nth in IHev2.
     econstructor; eauto. now rewrite -is_propositional_optimize.
+    eapply IHev2. admit.
   
   - now rewrite e.
 
-  - eapply Ee.eval_app_cong; eauto.
+  - move/andP => [] clf cla.
+    specialize (IHev1 clf). specialize (IHev2 cla).
+    eapply Ee.eval_app_cong; eauto.
     eapply Ee.eval_to_value in ev1.
     destruct ev1; simpl in *; eauto.
     * destruct t => //; rewrite optimize_mkApps /=.
@@ -452,6 +710,34 @@ Proof.
       rewrite orb_true_r /= // in i.
   - destruct t => //.
     all:constructor; eauto.
+Admitted.
+
+Lemma All2_All2_mix {A B} {P Q : A -> B -> Type} l l' : 
+  All2 P l l' ->
+  All2 Q l l' ->
+  All2 (fun x y => P x y × Q x y) l l'.
+Proof.
+  induction 1; intros H; depelim H; constructor; auto.
+Qed.
+
+Lemma erases_closed Σ Γ t t' : Σ;;; Γ |- t ⇝ℇ t' -> PCUICAst.closedn #|Γ| t -> closedn #|Γ| t'.
+Proof.
+  induction 1 using erases_forall_list_ind; cbn; auto; try solve [rtoProp; repeat solve_all].
+  - rtoProp. intros []. split; eauto. solve_all.
+    eapply Forall2_All2 in H1. eapply All2_All2_mix in X; tea.
+    eapply forallb_All in H3. eapply All2_All_mix_left in X; tea. clear H3.
+    clear H1.
+    solve_all. rewrite -b.
+    rewrite app_length inst_case_branch_context_length in a0.
+    eapply a0. now move/andP: a => [].
+  - unfold test_def in *. solve_all.
+    eapply All2_All2_mix in X; tea. solve_all.
+    len in a0. rewrite - (All2_length H).
+    eapply a0. now move/andP: a.
+  - unfold test_def in *. solve_all.
+    eapply All2_All2_mix in X; tea. solve_all.
+    len in a0. rewrite - (All2_length H).
+    eapply a0. now move/andP: a.
 Qed.
 
 Lemma erase_opt_correct (wfl := Ee.default_wcbv_flags) (Σ : global_env_ext) (wfΣ : wf_ext Σ) t v Σ' t' :
@@ -472,7 +758,9 @@ Proof.
   eapply erases_correct in ev; eauto.
   destruct ev as [v' [ev evv]].
   exists v'. split.
-  2:{ sq. now apply optimize_correct. }
+  2:{ sq. apply optimize_correct; tea.
+      clear HΣ'. eapply PCUICClosed.subject_closed in wt.
+      eapply erases_closed in H; tea. }
   auto. 
   rewrite <- Ht'.
   eapply erase_global_includes.
